src/Correctness/ForwardingCorrect.v
@@ -8,6 +8,7 @@ From Stdlib Require Import List Bool Lia PeanoNat.
 From coqutil Require Import Map.Interface Map.Properties Datatypes.ListSet Eqb Tactics.destr.
 From Datalog Require Import Map Default.
 From DatalogRocq Require Import DistributedDatalogToHardwareCompiler HardwareProgram DistributedHardwareProgram ComputableGraph.
+From GraphSearch Require Import GraphInterface.
 Import ListNotations.
 
 Section ForwardingCorrect.
@@ -15,10 +16,10 @@ Section ForwardingCorrect.
 Context {node_id : Type}.
 Context {node_id_eqb : Eqb node_id} {node_id_eqb_ok : Eqb_ok node_id_eqb}.
 Context {node_id_set : map.map node_id unit} {node_id_set_ok : map.ok node_id_set}.
-Context {node_id_edge_set : map.map node_id node_id_set} {node_id_edge_set_ok : map.ok node_id_edge_set}.
+Context {node_id_graph : graph.graph node_id} {node_id_graph_ok : graph.ok node_id_graph}.
 
-Notation node_graph := (@ComputableGraph.ComputableGraph node_id node_id_set node_id_edge_set).
-Notation cg_edge := (@ComputableGraph.cg_edge node_id node_id_set node_id_edge_set).
+Notation node_graph := (@ComputableGraph.ComputableGraph node_id node_id_set node_id_graph).
+Notation cg_edge := (@ComputableGraph.cg_edge node_id node_id_set node_id_graph).
 
 Context {forwarding_table : map.map (rel_id * node_id) (list node_id)}
         {forwarding_table_ok : map.ok forwarding_table}.
@@ -44,45 +45,26 @@ Definition has_fwd_edge (ftables : node_ftable_map) (node : node_id) (rel : rel_
 Definition ftable_edges_sound (g : node_graph) (ftables : node_ftable_map) : Prop :=
   forall node rel s m, has_fwd_edge ftables node rel s m -> cg_edge g node m.
 
-Lemma get_map_values {K V1 V2 : Type} {keqb : Eqb K} {keqb_ok : Eqb_ok keqb}
-    {M1 : map.map K V1} {M1ok : map.ok M1} {M2 : map.map K V2} {M2ok : map.ok M2}
-    (f : V1 -> V2) (m : M1) (k : K) :
-  map.get (map.map_values f m : M2) k = option_map f (map.get m k).
-Proof.
-  unfold map.map_values. revert k.
-  eapply (map.fold_spec (fun m acc => forall k, map.get (acc : M2) k = option_map f (map.get m k))).
-  - intros k. rewrite !map.get_empty. reflexivity.
-  - intros k v m' acc _ IH k0. rewrite !map.get_put_dec. destr (eqb k k0); [reflexivity | apply IH].
-Qed.
-
-Lemma get_node_set_of_list (l : list node_id) (m : node_id) :
-  map.get (DistributedDatalogToHardwareCompiler.node_set_of_list l : node_id_set) m <> None <-> In m l.
-Proof.
-  unfold DistributedDatalogToHardwareCompiler.node_set_of_list.
-  induction l as [|x l IH]; cbn [List.map map.of_list In].
-  - rewrite map.get_empty. split; [congruence | intros []].
-  - rewrite map.get_put_dec. destr (eqb x m).
-    + split; [intros _; left; reflexivity | congruence].
-    + rewrite IH. split; [tauto | intros [Heq|H]; [congruence | exact H]].
-Qed.
-
 (* an edge of the graph the table induces for [R] is exactly a recorded next hop *)
-Lemma cg_edge_graph_of_ftables (ftables : node_ftable_map) (R : rel_id) (s : node_id)
+Lemma edge_graph_of_ftables (ftables : node_ftable_map) (R : rel_id) (s : node_id)
     (n m : node_id) :
-  cg_edge (graph_of_ftables_at ftables R s) n m <-> has_fwd_edge ftables n R s m.
+  graph.edge (graph_of_ftables_at ftables R s) n m <-> has_fwd_edge ftables n R s m.
 Proof.
-  unfold ComputableGraph.cg_edge, ComputableGraph.check_edge_exists,
-    DistributedDatalogToHardwareCompiler.graph_of_ftables_at,
-    DistributedDatalogToHardwareCompiler.edges_of_ftables_at,
-    has_fwd_edge, node_rel_dests, get_or_default, get_or.
-  cbn [ComputableGraph.edges]. rewrite get_map_values.
-  destruct (map.get ftables n) as [ft|] eqn:Hn; cbn [option_map].
-  - rewrite <- get_node_set_of_list.
-    destruct (map.get (DistributedDatalogToHardwareCompiler.node_set_of_list _) m).
-    + split; [intros _; congruence | reflexivity].
-    + split; [discriminate | intros H; exfalso; apply H; reflexivity].
-  - cbv [default map_default list_default]. rewrite map.get_empty.
-    split; [discriminate | intros []].
+  unfold DistributedDatalogToHardwareCompiler.graph_of_ftables_at,
+    has_fwd_edge, node_rel_dests.
+  revert n m.
+  eapply (map.fold_spec
+    (fun m0 acc => forall n m, graph.edge acc n m
+                   <-> In m (get_or_default (get_or_default m0 n) (R, s)))).
+  - intros n m. unfold get_or_default, get_or. rewrite map.get_empty.
+    cbv [default map_default]. rewrite map.get_empty. cbv [list_default].
+    split; [apply graph.edge_empty | intros []].
+  - intros k v m0 acc Hk IH n m. rewrite graph.edge_put_edges, IH.
+    unfold get_or_default, get_or. rewrite map.get_put_dec.
+    destr (eqb k n).
+    + rewrite Hk. cbv [default map_default]. rewrite map.get_empty. cbv [list_default].
+      cbn [In]. tauto.
+    + split; [intros [H|[Hc _]]; [exact H | congruence] | intros H; left; exact H].
 Qed.
 
 (* the decidable check on an externally generated table gives exactly the edge-soundness the
@@ -98,7 +80,8 @@ Proof.
   destruct (map.get ft (rel, s)) as [hops|] eqn:Hrel; [|destruct Hfwd].
   pose proof (map.get_forallb _ ft Hft (rel, s) hops Hrel) as Hhops.
   unfold DistributedDatalogToHardwareCompiler.hops_in_graphb in Hhops.
-  rewrite forallb_forall in Hhops. exact (Hhops _ Hfwd).
+  rewrite forallb_forall in Hhops.
+  apply ComputableGraph.check_edge_exists_iff. exact (Hhops _ Hfwd).
 Qed.
 
 (*============================================================================*)
