src/DatalogCompilers/StringDatalog.v
@@ -4,10 +4,24 @@
    combine it with a topology backend (e.g. GridTopology) to get a concrete compiler. *)
 
 From DatalogRocq Require Import DistributedDatalogToHardwareCompiler StringDatalogParams.
-From coqutil Require Import Map.Interface Map.SortedListString.
+From coqutil Require Import Map.Interface Map.SortedListString Eqb Decidable.
+From GraphSearch Require Import GraphInterface GraphImpl.
 Import StringDatalogParams.
 
 (* Variables and functions are strings; these are the variable-keyed maps the compiler needs. *)
 #[global] Instance var_node_set : map.map _ _ := SortedListString.map unit.
-#[global] Instance var_edge_set : map.map _ _ := SortedListString.map (SortedListString.map unit).
+#[global] Instance var_eqb : Eqb string_var := String.eqb.
+
+#[global] Instance var_eqb_ok : Eqb_ok var_eqb.
+Proof. intros a b. unfold eqb, var_eqb. destruct (String.eqb_spec a b); assumption. Qed.
+
+#[global] Instance var_graph_impl : graph.graph string_var :=
+  @GraphImpl.graph_map string_var var_eqb var_eqb_ok
+    (SortedListString.map unit) (SortedListString.ok unit)
+    (SortedListString.map (SortedListString.map unit)) (SortedListString.ok _).
+
+#[global] Instance var_graph_impl_ok : graph.ok var_graph_impl :=
+  @GraphImpl.graph_map_ok string_var var_eqb var_eqb_ok
+    (SortedListString.map unit) (SortedListString.ok unit)
+    (SortedListString.map (SortedListString.map unit)) (SortedListString.ok _).
 #[global] Instance var_idx_map : map.map _ _ := SortedListString.map nat.
